\documentclass[12pt]{article}
\usepackage{ucs}
\usepackage[utf8x]{inputenc}
\usepackage[russian]{babel}
\title{\LaTeX}
\date{}
\author{}
\begin{document}
	\begin{center}
		\Large\textbf{Taking the derivative of a function}
	\end{center}
	Let $f(x) = $
	\begin{math}
<<<<<<< HEAD
		\exp{(x^2/2)}+\sin{(x^3+1)}*\tan{(\ln{(x^2+1)}+2)}\\
=======
		2*x/4\\
>>>>>>> 06b3f064458845b7c2e5f8842e0600251b173df9
	\end{math}
	\newline
	\newline
	Next, we will take the derivative $f^{'}_x(x)$:\newline
	\newline
	Step-by-step solution:\newline
	\begin{math}
<<<<<<< HEAD
		(\exp{(x^2/2)}+\sin{(x^3+1)}*\tan{(\ln{(x^2+1)}+2)})^{'}=(\sin{(x^3+1)}*\tan{(\ln{(x^2+1)}+2)})^{'}+(\exp{(x^2/2)})^{'}\\
((\sin{(x^3+1)})*(\tan{(\ln{(x^2+1)}+2)}))^{'}=(\sin{(x^3+1)})^{'}*(\tan{(\ln{(x^2+1)}+2)})+(\sin{(x^3+1)})*(\tan{(\ln{(x^2+1)}+2)})^{'}\\
\tan^{'}{(\ln{(x^2+1)}+2)}=1/\cos^{2}{(\ln{(x^2+1)}+2)}*(\ln{(x^2+1)}+2)^{'}\\
(\ln{(x^2+1)}+2)^{'}=2^{'}+(\ln{(x^2+1)})^{'}\\
\ln^{'}{(x^2+1)}=1/(x^2+1)*(x^2+1)^{'}\\
(x^2+1)^{'}=1^{'}+(x^2)^{'}\\
(x^{2})^{'}=x^{2-1}*(2*x^{'}+x*\ln{x}*2^{'})\\
\sin^{'}{(x^3+1)}=\cos{(x^3+1)}*(x^3+1)^{'}\\
(x^3+1)^{'}=1^{'}+(x^3)^{'}\\
(x^{3})^{'}=x^{3-1}*(3*x^{'}+x*\ln{x}*3^{'})\\
\exp^{'}{(x^2/2)}=\exp{(x^2/2)}*(x^2/2)^{'}\\
((x^2)/2)^{'}=((x^2)^{'}*2-(x^2)*2^{'})/2^2\\
(x^{2})^{'}=x^{2-1}*(2*x^{'}+x*\ln{x}*2^{'})\\
=======
		(2*(x/4))^{'}=2^{'}*(x/4)+2*(x/4)^{'}\\
(x/4)^{'}=(x^{'}*4-x*4^{'})/4^2\\
>>>>>>> 06b3f064458845b7c2e5f8842e0600251b173df9
	\end{math}
	\newline
	The derivative is:\newline
	\begin{math}
<<<<<<< HEAD
		\exp{(x^2/2)}*((x^{2-1}*(1*2+x*0*\ln{(x)})*2)-(0*x^2))/2^2+\cos{(x^3+1)}*(x^{3-1}*(1*3+x*0*\ln{(x)})+0)*\tan{(\ln{(x^2+1)}+2)}+1/(\cos{(\ln{(x^2+1)}+2)})^2*(1/(x^2+1)*(x^{2-1}*(1*2+x*0*\ln{(x)})+0)+0)*\sin{(x^3+1)}\\
=======
		0*x/4+((1*4)-(0*x))/4^2*2\\
>>>>>>> 06b3f064458845b7c2e5f8842e0600251b173df9
	\end{math}
	\newline
	But you can see many unnecessary actions.
	\newline
	Let us make some simplifications:\newline
	\begin{math}
<<<<<<< HEAD
		\exp{(x^2/2)}*((x*(1*2+x*0*\ln{(x)})*2)-(0*x^2))/2^2+\cos{(x^3+1)}*(x^{3-1}*(1*3+x*0*\ln{(x)})+0)*\tan{(\ln{(x^2+1)}+2)}+1/(\cos{(\ln{(x^2+1)}+2)})^2*(1/(x^2+1)*(x^{2-1}*(1*2+x*0*\ln{(x)})+0)+0)*\sin{(x^3+1)}\\
		\exp{(x^2/2)}*((x*(2+x*0)*2)-(0*x^2))/2^2+\cos{(x^3+1)}*(x^{3-1}*(1*3+x*0*\ln{(x)})+0)*\tan{(\ln{(x^2+1)}+2)}+1/(\cos{(\ln{(x^2+1)}+2)})^2*(1/(x^2+1)*(x^{2-1}*(1*2+x*0*\ln{(x)})+0)+0)*\sin{(x^3+1)}\\
		\exp{(x^2/2)}*((x*(2+0)*2)-(0*x^2))/4+\cos{(x^3+1)}*(x^{3-1}*(1*3+x*0*\ln{(x)})+0)*\tan{(\ln{(x^2+1)}+2)}+1/(\cos{(\ln{(x^2+1)}+2)})^2*(1/(x^2+1)*(x^{2-1}*(1*2+x*0*\ln{(x)})+0)+0)*\sin{(x^3+1)}\\
		\exp{(x^2/2)}*((x*2*2)-0)/4+\cos{(x^3+1)}*(x^{3-1}*(1*3+x*0*\ln{(x)})+0)*\tan{(\ln{(x^2+1)}+2)}+1/(\cos{(\ln{(x^2+1)}+2)})^2*(1/(x^2+1)*(x^{2-1}*(1*2+x*0*\ln{(x)})+0)+0)*\sin{(x^3+1)}\\
		\exp{(x^2/2)}*x*2*2/4+\cos{(x^3+1)}*(x^2*(1*3+x*0*\ln{(x)})+0)*\tan{(\ln{(x^2+1)}+2)}+1/(\cos{(\ln{(x^2+1)}+2)})^2*(1/(x^2+1)*(x^{2-1}*(1*2+x*0*\ln{(x)})+0)+0)*\sin{(x^3+1)}\\
		\exp{(x^2/2)}*x*2*2/4+\cos{(x^3+1)}*x^2*(3+x*0*\ln{(x)})*\tan{(\ln{(x^2+1)}+2)}+1/(\cos{(\ln{(x^2+1)}+2)})^2*(1/(x^2+1)*(x^{2-1}*(1*2+x*0*\ln{(x)})+0)+0)*\sin{(x^3+1)}\\
		\exp{(x^2/2)}*x*2*2/4+\cos{(x^3+1)}*x^2*(3+x*0)*\tan{(\ln{(x^2+1)}+2)}+1/(\cos{(\ln{(x^2+1)}+2)})^2*(1/(x^2+1)*(x^1*(1*2+x*0*\ln{(x)})+0)+0)*\sin{(x^3+1)}\\
		\exp{(x^2/2)}*x*2*2/4+\cos{(x^3+1)}*x^2*(3+0)*\tan{(\ln{(x^2+1)}+2)}+1/(\cos{(\ln{(x^2+1)}+2)})^2*(1/(x^2+1)*(x^1*(2+x*0*\ln{(x)})+0)+0)*\sin{(x^3+1)}\\
		\exp{(x^2/2)}*x*2*2/4+\cos{(x^3+1)}*x^2*3*\tan{(\ln{(x^2+1)}+2)}+(1/(x^2+1)*(x^1*(2+x*0*\ln{(x)})+0)+0)/(\cos{(\ln{(x^2+1)}+2)})^2*\sin{(x^3+1)}\\
		\exp{(x^2/2)}*x*2*2/4+\cos{(x^3+1)}*x^2*3*\tan{(\ln{(x^2+1)}+2)}+1/(x^2+1)*(x^1*(2+x*0*\ln{(x)})+0)/(\cos{(\ln{(x^2+1)}+2)})^2*\sin{(x^3+1)}\\
		\exp{(x^2/2)}*x*2*2/4+\cos{(x^3+1)}*x^2*3*\tan{(\ln{(x^2+1)}+2)}+(x^1*(2+x*0*\ln{(x)})+0)/(x^2+1)/(\cos{(\ln{(x^2+1)}+2)})^2*\sin{(x^3+1)}\\
		\exp{(x^2/2)}*x*2*2/4+\cos{(x^3+1)}*x^2*3*\tan{(\ln{(x^2+1)}+2)}+x^1*(2+x*0*\ln{(x)})/(x^2+1)/(\cos{(\ln{(x^2+1)}+2)})^2*\sin{(x^3+1)}\\
		\exp{(x^2/2)}*x*2*2/4+\cos{(x^3+1)}*x^2*3*\tan{(\ln{(x^2+1)}+2)}+x*(2+x*0*\ln{(x)})/(x^2+1)/(\cos{(\ln{(x^2+1)}+2)})^2*\sin{(x^3+1)}\\
		\exp{(x^2/2)}*x*2*2/4+\cos{(x^3+1)}*x^2*3*\tan{(\ln{(x^2+1)}+2)}+x*(2+x*0)/(x^2+1)/(\cos{(\ln{(x^2+1)}+2)})^2*\sin{(x^3+1)}\\
		\exp{(x^2/2)}*x*2*2/4+\cos{(x^3+1)}*x^2*3*\tan{(\ln{(x^2+1)}+2)}+x*(2+0)/(x^2+1)/(\cos{(\ln{(x^2+1)}+2)})^2*\sin{(x^3+1)}\\
		\exp{(x^2/2)}*x*2*2/4+\cos{(x^3+1)}*x^2*3*\tan{(\ln{(x^2+1)}+2)}+x*2/(x^2+1)/(\cos{(\ln{(x^2+1)}+2)})^2*\sin{(x^3+1)}\\
		\exp{(x^2/2)}*x*2*2/4+\cos{(x^3+1)}*x^2*3*\tan{(\ln{(x^2+1)}+2)}+x*2/(x^2+1)/(\cos{(\ln{(x^2+1)}+2)})^2*\sin{(x^3+1)}\\
	\end{math}
	\newline
	In this way:\newline
		\framebox{$f^{'}_x(x) = \exp{(x^2/2)}*x*2*2/4+\cos{(x^3+1)}*x^2*3*\tan{(\ln{(x^2+1)}+2)}+x*2/(x^2+1)/(\cos{(\ln{(x^2+1)}+2)})^2*\sin{(x^3+1)}$}\\	\newline
=======
		0+(4-(0*x))/4^2*2\\
		(4-(0*x))/16*2\\
		(4-0)/16*2\\
		4/16*2\\
		2/8*2\\
		2/4\\
		1/2\\
		1/2\\
	\end{math}
	\newline
	In this way:\newline
		\framebox{$f^{'}_x(x) = 1/2$}\\	\newline
>>>>>>> 06b3f064458845b7c2e5f8842e0600251b173df9
	Further simplifications reader can hold their own.\newline
\end{document}
